Introduce read_target operation, simplify assign_target to smt proofs

vera/VerilogToSMT/VerilogToSMTCorrect.v
@@ -91,6 +91,87 @@ Proof.
   simpl. apply SMTLib.value_eqb_eq.
 Qed.
 
+Equations read_target {w} (regs : RegisterState.t) (target : Verilog.assign_target w) : XBV.xbv w :=
+  read_target regs (Verilog.AssignVar var) := regs var;
+  read_target regs (Verilog.AssignBit loc _) :=
+    XBV.extr (regs (Location.var loc)) (Location.idx loc) 1;
+  read_target regs (Verilog.AssignSlice slice) :=
+    XBV.extr (regs (Slice.get_var slice)) (Slice.get_lo slice) w;
+  read_target regs (Verilog.AssignConcat lhs rhs) :=
+    XBV.concat (read_target regs lhs) (read_target regs rhs).
+
+Lemma assign_target_to_smt_value {w} tag (target : Verilog.assign_target w) :
+  forall ρ target_smt,
+    assign_target_to_smt tag target = inr target_smt ->
+    read_target (execution_of_valuation tag ρ) target =
+      XBV.from_bv (SMTLib.interp_term ρ target_smt).
+Proof.
+  induction target; intros * Htarget_smt;
+    simp assign_target_to_smt read_target in Htarget_smt |- *;
+    monad_inv; simpl.
+  - reflexivity.
+  - destruct loc as [vec idx]. cbn in *.
+    simp assign_target_to_smt in Htarget_smt. inv Htarget_smt.
+    unfold execution_of_valuation. simpl.
+    rewrite XBV.extr_no_exes by lia.
+    f_equal.
+    unfold smt_select_bit. simpl.
+    rewrite smtlib_interp_rewrite. simpl.
+    destruct_rew. reflexivity.
+  - dependent elimination slice.
+    simp assign_target_to_smt in Htarget_smt. inv Htarget_smt.
+    unfold execution_of_valuation. simpl.
+    change (XBV.extr (XBV.from_bv (ρ (verilog_to_smt_var tag var))) lo (1 + hi - lo) =
+      XBV.from_bv (BV.bv_extr lo (1 + hi - lo) (ρ (verilog_to_smt_var tag var)))).
+    apply XBV.extr_no_exes. lia.
+  - rewrite (IHtarget1 ρ t eq_refl).
+    rewrite (IHtarget2 ρ t0 eq_refl).
+    apply XBV.concat_no_exes.
+Qed.
+
+Lemma set_target_from_state {w} (target : Verilog.assign_target w) :
+  Verilog.assign_target_wf target ->
+  forall regs reference,
+    set_target regs target (read_target reference target)
+      =( Verilog.assign_target_writes target )=
+    reference.
+Proof.
+  intros Hwf.
+  induction Hwf; intros *; simp read_target set_target; simpl.
+  - intros [v bit_idx] Hloc.
+    apply LocationSet.of_variable_spec in Hloc. cbn in Hloc.
+    destruct Hloc as [Hv _]. subst v.
+    unfold RegisterState.get_location.
+    rewrite RegisterState.set_reg_get_in. reflexivity.
+  - intros loc' Hloc'.
+    apply LocationSet.singleton_spec in Hloc'. unfold LocationSet.E.eq in Hloc'. subst loc'.
+    unfold RegisterState.get_location, RegisterState.set_location.
+    rewrite RegisterState.set_reg_get_in, XBV.set_bit_get_in.
+    rewrite XBV.extr_bitOf by lia.
+    f_equal. lia.
+  - intros loc Hloc.
+    apply LocationSet.of_slice_spec in Hloc.
+    unfold Slice.has_location in Hloc. destruct Hloc as [Hvar Hidx].
+    unfold RegisterState.get_location, RegisterState.set_slice.
+    rewrite <- Hvar, RegisterState.set_reg_get_in.
+    replace (Location.idx loc) with
+      (Slice.get_lo slice + (Location.idx loc - Slice.get_lo slice))%N by lia.
+    rewrite XBV.set_slice_get_in by lia.
+    rewrite XBV.extr_bitOf.
+    + reflexivity.
+    + lia.
+    + apply Slice.wf_width.
+  - rewrite XBV.extr_concat_high, XBV.extr_concat_low.
+    apply RegisterState.match_on_split_union. split.
+    + apply IHHwf1.
+    + pose proof (IHHwf2 regs reference) as IHrhs.
+      intros loc Hloc.
+      transitivity (RegisterState.get_location
+        (set_target regs rhs (read_target reference rhs)) loc).
+      * exact (set_target_preserve lhs _ _ _ Hno_overlap loc Hloc).
+      * apply IHrhs. exact Hloc.
+Qed.
+
 Lemma assign_target_to_smt_valid {w} tag (target : Verilog.assign_target w) :
   Verilog.assign_target_wf target ->
   forall regs ρ target_smt,
@@ -101,60 +182,9 @@ Lemma assign_target_to_smt_valid {w} tag (target : Verilog.assign_target w) :
       (set_target regs target (XBV.from_bv (SMTLib.interp_term ρ target_smt)))
       ρ.
 Proof.
-  intros Hwf.
-  induction Hwf; intros * Htarget_smt;
-    simp assign_target_to_smt in Htarget_smt; monad_inv;
-    simp set_target; simpl.
-  - intros [v bit_idx] Hloc.
-    apply LocationSet.of_variable_spec in Hloc. cbn in Hloc.
-    destruct Hloc as [Hv _]. subst v.
-    unfold RegisterState.get_location, execution_of_valuation.
-    rewrite RegisterState.set_reg_get_in. reflexivity.
-  - destruct loc as [vec idx]. cbn in *.
-    simp assign_target_to_smt in Htarget_smt. inv Htarget_smt.
-    intros loc' Hloc'.
-    apply LocationSet.singleton_spec in Hloc'. unfold LocationSet.E.eq in Hloc'. subst loc'.
-    unfold RegisterState.get_location, RegisterState.set_location, execution_of_valuation.
-    rewrite RegisterState.set_reg_get_in, XBV.set_bit_get_in.
-    pose proof (smt_select_bit_value ρ (Var.varType vec) (var_to_smt tag vec) idx wf) as Hselect.
-    apply (f_equal (XBV.bitOf 0)) in Hselect.
-    simpl in Hselect.
-    change (XBV.bitOf 0
-      (XBV.from_bv (SMTLib.interp_term ρ (smt_select_bit (var_to_smt tag vec) idx)))
-      = XBV.bitOf idx (XBV.from_bv (ρ (verilog_to_smt_var tag vec)))).
-    rewrite <- Hselect. reflexivity.
-  - dependent elimination slice.
-    simp assign_target_to_smt in Htarget_smt. inv Htarget_smt.
-    intros loc Hloc.
-    apply LocationSet.of_slice_spec in Hloc.
-    unfold Slice.has_location in Hloc. cbn in Hloc.
-    destruct Hloc as [Hvar Hidx].
-    unfold RegisterState.get_location, RegisterState.set_slice, execution_of_valuation.
-    cbn [Slice.get_var Slice.get_lo].
-    rewrite <- Hvar, RegisterState.set_reg_get_in.
-    replace (Location.idx loc) with (lo + (Location.idx loc - lo))%N by lia.
-    change (lo <= Location.idx loc < lo + (1 + hi - lo))%N in Hidx.
-    assert (Hoff : (Location.idx loc - lo < 1 + hi - lo)%N) by lia.
-    rewrite XBV.set_slice_get_in by exact Hoff.
-    simpl.
-    change (XBV.bitOf (Location.idx loc - lo)
-      (XBV.from_bv (BV.bv_extr lo (1 + hi - lo) (ρ (verilog_to_smt_var tag var)))) =
-      XBV.bitOf (lo + (Location.idx loc - lo))
-        (XBV.from_bv (ρ (verilog_to_smt_var tag var)))).
-    rewrite <- XBV.extr_no_exes by lia.
-    rewrite XBV.extr_bitOf by lia.
-    f_equal.
-  - rewrite <- XBV.concat_no_exes.
-    apply verilog_smt_match_states_partial_split_iff. split.
-    + rewrite XBV.extr_concat_high.
-      apply IHHwf1. reflexivity.
-    + rewrite XBV.extr_concat_low.
-      pose proof (IHHwf2 regs ρ t0 eq_refl) as IHrhs.
-      intros loc Hloc.
-      transitivity (RegisterState.get_location
-        (set_target regs rhs (XBV.from_bv (SMTLib.interp_term ρ t0))) loc).
-      * exact (set_target_preserve lhs _ _ _ Hno_overlap loc Hloc).
-      * apply IHrhs. exact Hloc.
+  intros Hwf * Htarget_smt.
+  rewrite <- (assign_target_to_smt_value tag target ρ target_smt Htarget_smt).
+  apply set_target_from_state. exact Hwf.
 Qed.
 
 Lemma module_item_to_smt_valid tag  (mi : Verilog.module_item) :
